cosmetic changes

website/Walkthrough/Blog/_5_AddingGoalsAndHypotheses.lean
@@ -7,7 +7,7 @@ open Verso Genre Blog
 ```leanInit AGH
 ```
 
-By the end of this section, you'll create a version of the `apply` tactic.
+By the end of this section, you'll create a version of the `apply` tactic.  This tactic "applies" a lemma which has a conclusion that matches the current goal, and updates the current goal accordingly.
 
 We will begin by writing tactics to access and modify the goals in the tactic state.
 
@@ -73,9 +73,8 @@ We will now look at modifying the tactic state beyond just manipulating the list
 We can extract out the basics of goal creation into a helper tactic: `createGoal`.
 
 ```lean AGH
-open Lean Elab Meta Tactic
-
-def createGoal (goalType : Expr) : TacticM Unit := withMainContext do
+def createGoal (goalType : Expr) : TacticM Unit :=
+withMainContext do
   let goal ← mkFreshExprMVar goalType
   appendGoals [goal.mvarId!]
 ```
@@ -109,7 +108,9 @@ example : 1 + 2 = 3 := by
   simp; simp
 ```
 
-We can also modify the syntax of the tactic to include the type of the new goal as a parameter.
+Until now, we had to be in an `elab` to decide what goal would be created.
+
+But now, we can create a tactic that allows us to decide what the new goal is from within the proof itself.
 
 ```lean AGH
 elab "create_goal" t:term : tactic => do
@@ -121,14 +122,25 @@ example : 1 + 2 = 3 := by
   simp; exact Nat.prime_two
 ```
 
+
+
 # Adding a new hypothesis
 
 Similarly, we can extract out the basics of hypothesis creation into a helper tactic: `createHypothesis`.
 
 ```lean AGH
-def createHypothesis (hypType : Expr) (hypProof : Expr) (hypName := `h) : TacticM Unit := do
-  let hyp : Hypothesis := { userName := hypName, type := hypType, value := hypProof }
-  let (_, new_goal) ← (← getMainGoal).assertHypotheses (List.toArray [hyp])
+def createHypothesis
+  (hypType : Expr) (hypProof : Expr) (hypName := `h) :
+  TacticM Unit :=
+do
+  let hyp : Hypothesis := {
+    userName := hypName,
+    type := hypType,
+    value := hypProof
+  }
+  let (_, new_goal) ← (← getMainGoal).assertHypotheses (
+    List.toArray [hyp]
+  )
   setGoals [new_goal]
 ```
 
@@ -136,8 +148,8 @@ Here’s an example of adding a hypothesis that looks like `h : ℕ`.
 
 ```lean AGH
 elab "create_nat_hypothesis" : tactic => do
-  let hypType := Expr.const ``Nat []
-  let hypProof := (toExpr 0) -- use 0 as a term of type Nat
+  let hypType := Expr.const ``Nat [] -- type of Nat
+  let hypProof := (toExpr 0) -- term of 0
   createHypothesis hypType hypProof
 
 example : 1 + 2 = 3 := by
@@ -149,8 +161,8 @@ Here’s an example of adding a hypothesis that is a proposition `0 = 0`.
 
 ```
 elab "create_reflexivity_hypothesis" : tactic => do
-  let hypType ← mkEq (toExpr 0) (toExpr 0) -- make the metavariable goal to prove that "0 = 0"
-  let hypProof ← mkAppM ``Eq.refl #[toExpr 0] -- proof that Eq 0 0
+  let hypType ← mkEq (toExpr 0) (toExpr 0) -- statement that "0 = 0"
+  let hypProof ← mkAppM ``Eq.refl #[toExpr 0] -- proof that "0 = 0"
   createHypothesis hypType hypProof
 
 example : 1 + 2 = 3 := by
@@ -164,17 +176,17 @@ Lean will technically let us create bogus hypotheses.
 
 ```lean AGH
 elab "create_bogus_hypothesis" : tactic => do
-  let hypType ← mkEq (toExpr 0) (toExpr 1) -- make the metavariable goal to prove that "0 = 0"
-  let hypProof  ← mkAppM ``Eq.refl #[toExpr 0] -- proof that Eq 0 0
+  let hypType ← mkEq (toExpr 0) (toExpr 1)  -- statement that "0 = 1"
+  let hypProof  ← mkAppM ``Eq.refl #[toExpr 0] -- proof that "0 = 0"
   createHypothesis hypType hypProof
 ```
 
 ```lean AGH
 example : 0=1 := by
-  create_bogus_hypothesis -- a new bogus hypothesis in the context
+  create_bogus_hypothesis -- "0=1" is now a hypothesis
   sorry
 ```
-But, if we actually try to use that hypothesis to prove a theorem, it will throw an error
+But, if we actually try to use that hypothesis to prove a theorem, it will throw a low-level error in the kernel.  A similar thing occurred previously with `setGoals`, where we could drop all active goals from the tactic state, but we got a kernel error if we tried to then finish the proof.
 
 ```lean AGH error:=true
 example : 0=1 := by
@@ -182,21 +194,29 @@ example : 0=1 := by
   assumption
 ```
 
-The issue here is that the tactic isn't checking the hypothesis statement matches the proof …
+Ideally, we want to catch this error earlier.
 
-That is, by propositions-as-types and proofs-as-terms, the inferred type of the proof should be the type.
+To do that, we want our tactic to check that the hypothesis statement matches the proof. That is, by propositions-as-types and proofs-as-terms, the inferred type of the `hypProof` should be `hypType`.
 
-A similar thing occurred previously with `setGoals`, where we could drop all active goals from the tactic state.
-
-So let's modify our `createHypothesis` function to check that ...
+So let's modify our `createHypothesis` function to perform this check.
 
 ```lean AGH
-def createHypothesisGuarded (hypType : Expr) (hypProof : Expr) : TacticM Unit := do
-  let hypName := `h
+def createHypothesisGuarded
+  (hypType : Expr) (hypProof : Expr) (hypName := `h):
+  TacticM Unit :=
+do
   unless ← isDefEq hypType (← inferType hypProof) do
-    throwError "The proof used for creating the hypothesis does not match the expected type."
-  let hyp : Hypothesis := { userName := hypName, type := hypType, value := hypProof }
-  let (_, new_goal) ← (← getMainGoal).assertHypotheses (List.toArray [hyp])
+    throwError
+      "The proof used for creating the hypothesis
+      does not match the expected type."
+  let hyp : Hypothesis := {
+    userName := hypName,
+    type := hypType,
+    value := hypProof
+  }
+  let (_, new_goal) ← (← getMainGoal).assertHypotheses (
+    List.toArray [hyp]
+  )
   setGoals [new_goal]
 ```
 
@@ -205,31 +225,31 @@ Here, the `inferType` function is used to deduce the type of `hypProof` (or the 
 Adding the bogus hypothesis no longer works with the `createHypothesisGuarded` function.
 
 ```lean AGH error := true
-elab "create_bogus_hypothesis" : tactic => do
-  let hypType ← mkEq (toExpr 0) (toExpr 1) -- make the metavariable goal to prove that "0 = 0"
-  let hypProof  ← mkAppM ``Eq.refl #[toExpr 0] -- proof that Eq 0 0
+elab "create_bogus_hypothesis'" : tactic => do
+  let hypType ← mkEq (toExpr 0) (toExpr 1) -- statement that "0 = 1"
+  let hypProof  ← mkAppM ``Eq.refl #[toExpr 0] -- proof that "0 = 0"
   createHypothesisGuarded hypType hypProof
 
 example : 0=1 := by
-  create_bogus_hypothesis
+  create_bogus_hypothesis'
   assumption
 ```
 
-# Adding a library result as a hypothesis
+# Adding a known theorem as a hypothesis
 
-We've previously seen that it's possible to retrieve the statement and proof of a library theorem from the environment given its name.
+We've previously seen that it's possible to retrieve the statement and proof of a theorem from the environment given its name.
 
-As an easy application of the tools we've developed so far, let's write a tactic that takes the name of a library result and adds it as a local hypothesis.
+As an easy application of the tools we've developed so far, let's write a tactic that takes the name of a theorem in the environment and adds it as a local hypothesis.
 
 ```lean AGH
-elab "add_library_hypothesis" nm:name : tactic => do
+elab "add_theorem_as_hypothesis" nm:name : tactic => do
   let some thm := (← getEnv).find? nm.getName |
     throwError s!"The result {nm} is not in the environment."
   createHypothesisGuarded thm.type thm.value!
 
-example : 1 + 2 = 3 := by
-  add_library_hypothesis `Nat.add_comm
-  rfl
+example : 1 + 2 = 2 + 1 := by
+  add_theorem_as_hypothesis `Nat.add_comm -- adds "h"
+  exact (h 1 2)
 ```
 
 # Making progress on a proof state
@@ -244,7 +264,7 @@ So far, we have written tactics that work on the list of active goals or add hyp
 
 For example, suppose the goal is to prove that `2 ^ 3` is not a prime number. The library contains the result `Nat.Prime.not_prime_pow`, which says that if `x` and `n` are natural numbers and `2 ≤ n`, then `x ^ n` is not a prime number.
 
-A mathematician would say "to show that `2 ^ 3` is not prime, it is sufficient to show that `2 ≤ 3`, by the result `Nat.Prime.not_prime_pow`." (except maybe for the last bit); the `apply` tactic is a way to formally mirror this style of reasoning in Lean.
+A mathematician would say "to show that `2 ^ 3` is not prime, it is sufficient to show that `2 ≤ 3`, by the result `Nat.Prime.not_prime_pow`." (except maybe for the last bit). The `apply` tactic is a way to formally mirror this style of reasoning in Lean.
 
 ```lean AGH
 #check Nat.Prime.not_prime_pow
@@ -259,32 +279,43 @@ We'll start with the scenario where we have a goal `Q` and a local hypothesis of
 
 Our rough strategy is going to be to:
 - Check whether the hypothesis is an implication, i.e., of the form `P → Q`
-- Check whether the conclusion of the hypothesis matches the type of the current goal
+- Check whether the conclusion of the hypothesis `h` matches the type of the current goal
 - Create a new goal `p` of type `P`
-- Assign the value `h p` to the current goal, where `h` is the hypothesis
+- Assign the value `h p` to the current goal (remember `h` is of form `P → Q`, so `h p` is of form `Q`)
 - Set `p` as the main goal
 
 Here is what this strategy looks like translated into code (parts of this code are deliberately sub-optimal; we'll see ways of improving it shortly):
 
 ```lean AGH
-elab "apply_hypothesis" h:term : tactic => withMainContext do
+elab "apply_hypothesis" h:term : tactic =>
+withMainContext do
   -- read the local context
   let lctx ← getLCtx
-  -- retrieve the `fvarId` corresponding to the local hypothesis `h`
+
+  -- retrieve the variable for local hypothesis `h`
   let fvarId ← getFVarId h
+
   -- retrieve the declaration for `h` from the local context
-  let some hyp := lctx.find? fvarId | throwError "Failed to find hypothesis in context."
+  let some hyp := lctx.find? fvarId |
+    throwError "Failed to find hypothesis in context."
+
   -- ensure that the hypothesis is an implication
   guard hyp.type.isArrow
-  -- extract the antecedent and the consequent of the implication
+
+  -- extract the implication's antecedent & consequent
   let .forallE _ P Q _ := hyp.type | unreachable!
-  -- ensure that the conclusion of `h` matches the current target
+
+  -- ensure that the conclusion of `h` matches the target
   unless Q == (← getMainTarget) do
-    throwError m!"The type of the conclusion of {h} does not match the current target."
+    throwError m!"The type of the conclusion of {h}
+    does not match the current target."
+
   -- create a new goal of type `P`
   let newGoal ← mkFreshExprMVar P
+
   -- assign the value `h newGoal` to the current goal
   (← getMainGoal).assign (.app hyp.toExpr newGoal)
+
   -- set `newGoal` as the main goal
   replaceMainGoal [newGoal.mvarId!]
 
@@ -305,37 +336,49 @@ We get a type mismatch error since Lean can't tell that `Even 4` is the same as 
 The error goes away when we switch to the coarser notion of "definitional equality" (checked by the function `isDefEq`):
 
 ```lean AGH
-elab "apply_hypothesis_defeq" h:term : tactic => withMainContext do
+elab "apply_hypothesis_defeq" h:term : tactic =>
+withMainContext do
   -- read the local context
   let lctx ← getLCtx
-  -- retrieve the `fvarId` corresponding to the local hypothesis `h`
+
+  -- retrieve the variable for local hypothesis `h`
   let fvarId ← getFVarId h
+
   -- retrieve the declaration for `h` from the local context
-  let some hyp := lctx.find? fvarId | throwError "Failed to find hypothesis in context."
+  let some hyp := lctx.find? fvarId |
+    throwError "Failed to find hypothesis in context."
+
   -- ensure that the hypothesis is an implication
   guard hyp.type.isArrow
-  -- extract the antecedent and the consequent of the implication
+
+  -- extract the implication's antecedent & consequent
   let .forallE _ P Q _ := hyp.type | unreachable!
-  -- ensure that the conclusion of `h` matches the current target
+
+  -- ensure that the conclusion of `h` matches the target
   unless ← isDefEq Q (← getMainTarget) do
-    throwError m!"The type of the conclusion of {h} does not match the current target."
+    throwError m!"The type of the conclusion of {h}
+    does not match the current target."
+
   -- create a new goal of type `P`
   let newGoal ← mkFreshExprMVar P
+
   -- assign the value `h newGoal` to the current goal
   (← getMainGoal).assign (.app hyp.toExpr newGoal)
+
   -- set `newGoal` as the main goal
   replaceMainGoal [newGoal.mvarId!]
-
+```
+Now the example works as intended.
+```lean AGH
 example (h : Even 2 → Even 4) : Even (2 * 2) := by
   apply_hypothesis_defeq h -- the goal is now `Even 2`
   rw [even_iff_two_dvd]
 ```
+# Unification
 
-# Meta-variables and unification
+As mentioned before, the function `isDefEq` does more than just checking for definitional equality - it also handles the *unification* (roughly, filling in holes) of *expressions containing meta-variables* (roughly, expressions with holes).
 
-The function `isDefEq` does more than just checking for definitional equality - it also handles the *unification* of *expressions containing meta-variables* (i.e., expressions with holes).
-
-For example, consider the two expressions `(_ * 37)` and `(71 * _)`, where the underscores indicate "holes" in the expressions. While these expressions are not equal on the nose, they can be made equal by choosing the values for the holes appropriately (so that they both become `71 * 37`). This is the idea behind *unification*, and the `isDefEq` function tries to fill in the holes as much as possible to make the two expressions match up.
+For example, consider the two expressions `(_ * 37)` and `(71 * _)`, where the underscores indicate "holes" in the expressions. While these expressions are not equal by `==`, they are by `isDefEq`, since they can be made equal by choosing the values for the holes appropriately (so that they both become `71 * 37`). This is the idea behind *unification*, and the `isDefEq` function tries to fill in the holes as much as possible to make the two expressions match up.
 
 The word *meta-variable* was used earlier in a different sense - to refer to a goal in the tactic. However, the two senses of the word are essentially the same - a goal can be thought of as a hole for a proof of the appropriate type.
 
@@ -344,36 +387,49 @@ We can implement the `apply_hypothesis` using a strategy involving unification:
 - Create a meta-variable `?P` for the type of the new goal
 - Check whether the type of the hypothesis unifies with the expression `?P → Q`
 - If the unification succeeds and the meta-variable `?P` is assigned the value `P`, create a meta-variable `p` of type `P` for the new goal
-- Assign the value `h p` to the current goal, where `h` is the hypothesis
+- Assign the value `h p` to the current goal
 - Set `p` as the main goal
+
+With this approach, we no longer need to check if the hypothesis is an implication and explicitly extracting its antecedent and consequent.
 
 ```lean AGH
 
 elab "apply_hypothesis_unif" h:term : tactic => withMainContext do
-  -- the type of the main goal
-  let currentTarget ← getMainTarget
-  -- a meta-variable for the type of the new goal
-  let newTarget ← mkFreshExprMVar none
   -- read the local context
   let lctx ← getLCtx
-  -- retrieve the `fvarId` corresponding to the local hypothesis `h`
+
+  -- retrieve the variable for local hypothesis `h`
   let fvarId ← getFVarId h
+
   -- retrieve the declaration for `h` from the local context
-  let some hyp := lctx.find? fvarId | throwError "Failed to find hypothesis in context."
-  -- attempt to unify the type of the hypothesis with `newTarget → currentTarget`
+  let some hyp := lctx.find? fvarId |
+    throwError "Failed to find hypothesis in context."
+
+  -- try to unify hypothesis with `newTarget → currentTarget`
+  let currentTarget ← getMainTarget
+  let newTarget ← mkFreshExprMVar none
   unless ← isDefEq hyp.type (← mkArrow newTarget currentTarget) do
-    throwError m!"The hypothesis is expected to be an implication with conclusion matching the current goal."
-  -- replace `newTarget` with the concrete value determined through unification
+    throwError m!"The hypothesis is expected to be an implication
+      with conclusion matching the current goal."
+
+  -- fill in holes in `newTarget`
   let newTarget ← instantiateMVars newTarget
-  -- logging information about the type of the new goal
-  logInfo m!"The new target is {newTarget}."
+
   -- create a new goal of type `newTarget`
   let newGoal ← mkFreshExprMVar newTarget
+
+  -- logging information about the type of the new goal
+  logInfo m!"The new target was updated from {currentTarget} to {newTarget}."
+
   -- assign the value `h newGoal` to the current goal
   (← getMainGoal).assign (.app hyp.toExpr newGoal)
+
   -- set `newGoal` as the main goal
   replaceMainGoal [newGoal.mvarId!]
+```
 
+And the tactic works the same as before.
+```lean AGH
 example (h : Even 2 → Even 4) : Even (2 * 2) := by
   apply_hypothesis_unif h
   rw [even_iff_two_dvd]
@@ -381,7 +437,7 @@ example (h : Even 2 → Even 4) : Even (2 * 2) := by
 
 # A more general `apply` tactic
 
-To finish off this chapter, we'll generalize our `apply_hypothesis` tactic to scenarios where the type of the argument is not just a single implication arrow.
+To finish off this chapter, we'll generalize our `apply_hypothesis` tactic to scenarios where the type of the argument is not just a single implication.
 
 For example, suppose we have a target like `¬Nat.Prime (2 * 3)` that we want to prove by backwards reasoning using `Nat.not_prime_mul` (shown below), which says that the product of two numbers is not prime when those numbers are both not equal to 1.
 
